wip low-level Merkle tree implementation

examples/low-level/merkletree/c/merkle_tree.h
@@ -3,6 +3,15 @@
 
 typedef uint8_t[32] hash_t;
 typedef uint8_t *path_t;
+
+typedef struct merkle_tree_s
+{
+  uint32_t nelts;
+  hash_t *values;
+  hash_t *iroots;
+}
+  merkle_tree;
+  
 typedef merkle_tree *mt_ptr;
 
 mt_ptr create();
