examples/low-level/merkletree/MerkleTree.Low.fst
@@ -1,12 +1,14 @@
 module MerkleTree.Low
 
-open MerkleTree.High
+// open MerkleTree.High
+// open EverCrypt.Hash
 
 open FStar.All
 open FStar.Mul
 open LowStar.Modifies
 open LowStar.BufferOps
 open FStar.Seq
+open FStar.Integers
 
 module List = FStar.List.Tot
 module HS = FStar.HyperStack
@@ -14,180 +16,146 @@ module HST = FStar.HyperStack.ST
 module B = LowStar.Buffer
 module S = FStar.Seq
 
-module High = MerkleTree.High
+// module High = MerkleTree.High
 
 let root = Monotonic.HyperHeap.root
-let elem_buf = B.buffer elem
+
+type uint32_t = UInt32.t
+type uint8_t = UInt8.t
+
+let hash_size = 32
+type hash = b:B.buffer uint8_t{B.length b = hash_size}
 let hash_buf = B.buffer hash
 
-// This number says that the maximum number of values is (2^32 - 1)
-unfold let max_nelts_sz = 32
+// assume val hash_from_hashes: 
+//   src1:hash -> src2:hash -> dst:hash -> 
+//   HST.St unit
+// 	 (requires (fun h0 -> 
+// 	   B.live h0 src1 /\ B.live h0 src2 /\ B.live h0 dst))
+// 	 (ensures (fun h0 _ h1 ->
+// 	   modifies (loc_addr_of_buffer
 
-/// Allocation by power of two
+/// Utilities
 
-val alloc_sz_lg:
-  nelts:nat{nelts > 0} -> 
-  GTot (sz:nat{sz > 0 && pow2 (sz - 1) <= nelts && nelts < pow2 sz})
-let rec alloc_sz_lg nelts = pow2_floor nelts + 1
+val uint32_pow2: sz:uint32_t{sz < 32ul} -> Tot uint32_t
+let rec uint32_pow2 sz =
+  UInt32.shift_left 1ul sz
 
-unfold val alloc_sz: nelts:nat{nelts > 0} -> GTot nat
-unfold let alloc_sz nelts =
-  pow2 (alloc_sz_lg nelts) - 1
+val uint32_is_pow2: uint32_t -> Tot bool
+let rec uint32_is_pow2 n =
+  n <> 0ul && UInt32.logor n (n -% 1ul) = 0ul
 
-val alloc_sz_lg_pow2_inc:
-  nelts:nat{nelts > 0} ->
-  Lemma (requires (is_pow2 (nelts + 1)))
-	(ensures (alloc_sz_lg (nelts + 1) = 1 + alloc_sz_lg nelts))
-let rec alloc_sz_lg_pow2_inc nelts =
-  if nelts = 1 then ()
-  else alloc_sz_lg_pow2_inc (nelts / 2)
+val uint32_pow2_floor: n:uint32_t{n > 0ul} -> 
+  Tot (p:uint32_t{p < 32ul && uint32_pow2 p <= n})
+let uint32_pow2_floor n = admit ()
 
-val alloc_sz_lg_not_pow2_inc:
-  nelts:nat{nelts > 0} ->
-  Lemma (requires (~ (is_pow2 (nelts + 1))))
-	(ensures (alloc_sz_lg nelts = alloc_sz_lg (nelts + 1)))
-let alloc_sz_lg_not_pow2_inc nelts =
-  let sz1 = alloc_sz_lg nelts in
-  let sz2 = alloc_sz_lg (nelts + 1) in
-  if sz1 > sz2 
-  then Math.Lemmas.pow2_le_compat (sz1 - 1) sz2
-  else if sz1 < sz2
-  then (Math.Lemmas.pow2_le_compat (sz2 - 1) sz1;
-       assert (nelts = pow2 sz1))
-  else ()
+/// Hash pointers
+
+// val copy_hash: src:hash -> dst:hash -> HST.St unit
+// let copy_hash src dst =
+//   B.upd dst 0ul (B.index src 0ul)
+//     B.upd (B.index nvs nelts) 0ul (B.index e 0ul);
+
+
 
 /// Low-level Merkle tree data structure
 
 noeq type merkle_tree =
-| MT: nelts:nat{nelts > 0 && nelts < pow2 max_nelts_sz} -> 
+| MT: nelts:uint32_t{nelts > 0ul} -> 
       // The value buffer will be resized when elements are added.
       // Resizing mechanism will be similar to that of C++ vector.
-      values:elem_buf{B.length values = alloc_sz nelts} ->
+      values:hash_buf ->
       // The actual number of internal roots should be equal to 
       // the number of "set" bits of `nelts`.
-      iroots:hash_buf{B.length iroots = max_nelts_sz} ->
+      iroots:hash_buf ->
       merkle_tree
 
 let mtree_ptr = B.pointer merkle_tree
 
-val num_iroots_of_bound: 
-  nelts_sz:nat -> nelts:nat{nelts < pow2 nelts_sz} -> 
-  GTot (nirs:nat{nirs = num_iroots_of nelts && nirs <= nelts_sz})
-let rec num_iroots_of_bound nelts_sz nelts =
-  if nelts = 0 then 0
-  else 1 + num_iroots_of_bound (nelts_sz - 1) (nelts - pow2 (pow2_floor nelts))
-
-unfold val merkle_tree_wf: HS.mem -> merkle_tree -> GTot Type0
-unfold let merkle_tree_wf h mt =
-  let nelts = MT?.nelts mt in
-  let vs = MT?.values mt in
-  let irs = MT?.iroots mt in
-  B.live h vs /\ B.freeable vs /\ B.live h irs /\ B.disjoint vs irs /\
-  iroots_of (S.slice (B.as_seq h vs) 0 nelts) =
-  S.slice (B.as_seq h irs) 0 (num_iroots_of_bound max_nelts_sz nelts)
-
-val merkle_tree_lift: 
-  h:HS.mem -> mt:merkle_tree{merkle_tree_wf h mt} -> GTot (High.merkle_tree)
-let merkle_tree_lift h mt =
-  High.MT (S.slice (B.as_seq h (MT?.values mt)) 0 (MT?.nelts mt))
-	  (S.slice (B.as_seq h (MT?.iroots mt))
-		   0 (num_iroots_of_bound max_nelts_sz (MT?.nelts mt)))
-
 /// Initialization
 
-val create_merkle_tree: unit -> 
-  HST.ST merkle_tree
-	 (requires (fun _ -> true))
-	 (ensures (fun h0 mt h1 -> merkle_tree_wf h1 mt))
-let create_merkle_tree _ = 
-  let values = B.malloc root elem_init 1ul in
-  let hh0 = HST.get () in
-  let iroots = B.malloc root (hash_from_elem elem_init) (UInt32.uint_to_t max_nelts_sz) in
-  let hh1 = HST.get () in
-  B.live_unused_in_disjoint hh0 values iroots;
-  S.lemma_eq_intro (iroots_of (S.slice (B.as_seq hh1 values) 0 1))
-  		   (S.slice (B.as_seq hh1 iroots) 0 1);
-  MT 1 values iroots
 
-val create: unit -> HST.St mtree_ptr
-let create _ = B.malloc root (create_merkle_tree ()) 1ul
+
+val create_hashes: 
+  idx:uint32_t -> len:uint32_t -> 
+  hs:B.buffer hash{UInt32.v idx < B.length hs} ->
+  HST.ST unit
+	 (requires (fun h0 -> B.live h0 hs))
+	 (ensures (fun h0 _ h1 -> modifies (loc_buffer hs) h0 h1))
+let rec create_hashes idx len hs =
+  if len = 0ul then ()
+  else (B.upd hs idx (B.malloc root (UInt8.uint_to_t 0) hash_size);
+       assume (UInt32.v (idx + 1ul) < B.length hs);
+       create_hashes (idx + 1ul) (len - 1ul) hs)
+
+val create_merkle_tree: unit -> 
+  HST.ST mtree_ptr
+	 (requires (fun _ -> true))
+	 (ensures (fun h0 mt h1 -> true))
+let create_merkle_tree _ = 
+  let values = B.malloc root B.null 1ul in
+  create_hashes 0ul 1ul values;
+  let iroots = B.malloc root B.null 32ul in
+  create_hashes 0ul 32ul iroots;
+  B.malloc root (MT 1ul values iroots) 1ul
 
 /// Insertion
 
-val mt_is_full: merkle_tree -> Tot bool
-let mt_is_full mt = MT?.nelts mt >= pow2 max_nelts_sz - 1
-
-val insert_nelts: 
-  nelts:nat{nelts < pow2 max_nelts_sz - 1} ->
-  Tot (inelts:nat{inelts < pow2 max_nelts_sz})
-let insert_nelts nelts =
-  nelts + 1
-
 val insert_values:
-  nelts:nat{nelts > 0 && nelts < pow2 max_nelts_sz - 1} -> 
-  vs:elem_buf{B.length vs = alloc_sz nelts} ->
-  e:elem -> 
-  HST.ST (ivs:elem_buf{B.length ivs = alloc_sz (insert_nelts nelts)})
+  nelts:uint32_t{nelts > 0ul} -> 
+  vs:hash_buf ->
+  e:hash -> 
+  HST.ST (ivs:hash_buf)
 	 (requires (fun h0 -> B.live h0 vs /\ B.freeable vs))
-	 (ensures (fun h0 nvs h1 -> 
-	   B.live h1 nvs /\ B.freeable nvs /\
-	   S.slice (B.as_seq h1 nvs) 0 (insert_nelts nelts) ==
-	   High.insert_values (S.slice (B.as_seq h0 vs) 0 nelts) e))
-#set-options "--z3rlimit 40"
+	 (ensures (fun h0 nvs h1 -> B.live h1 nvs /\ B.freeable nvs))
+#set-options "--z3rlimit 10"
 let insert_values nelts vs e =
-  if is_pow2 (nelts + 1)
-  then (let hh0 = HST.get () in
-       // Need to prove `2 * nelts + 1` does not exceed the maximum before `B.malloc`
-       pow2_lt_le (nelts + 1) max_nelts_sz; 
-       let nvs = B.malloc root elem_init (UInt32.uint_to_t (2 * nelts + 1)) in
-
+  if uint32_is_pow2 (nelts +% 1ul)
+  then (let nvs = B.malloc root B.null (2ul * (nelts + 1ul)) in
        // `blit` requires two buffers to be disjoint
-       B.live_unused_in_disjoint hh0 vs nvs;
-       loc_disjoint_buffer vs nvs;
-       LowStar.BufferOps.blit vs 0ul nvs 0ul (UInt32.uint_to_t nelts);
+       LowStar.BufferOps.blit vs 0ul nvs 0ul nelts;
+       create_hashes (nelts + 1ul) (nelts + 1ul) nvs;
+       B.upd (B.index nvs nelts) 0ul (B.index e 0ul);
 
-       B.upd nvs (UInt32.uint_to_t nelts) e;
-       let hh1 = HST.get () in
-       S.lemma_eq_elim (S.slice (B.as_seq hh1 nvs) 0 (insert_nelts nelts))
-       		       (High.insert_values (S.slice (B.as_seq hh0 vs) 0 nelts) e);
-
-       // TODO: should be able to prove that `nvs` is not affected after `B.free`
-       // there might be a relation among `B.disjoint`, `B.free`, and `B.live`
-       // B.free vs;
-       // let hh2 = HST.get () in assume (B.live hh2 nvs);
-
-       alloc_sz_lg_pow2_inc nelts;
+       B.free vs;
+       let hh2 = HST.get () in assume (B.live hh2 nvs);
        nvs)
-  else (let hh0 = HST.get () in
-       B.upd vs (UInt32.uint_to_t nelts) e; 
-       let hh1 = HST.get () in
-       S.lemma_eq_elim (S.slice (B.as_seq hh1 vs) 0 (insert_nelts nelts))
-       		       (High.insert_values (S.slice (B.as_seq hh0 vs) 0 nelts) e);
-       alloc_sz_lg_not_pow2_inc nelts;
-       vs)
+  else (assume (UInt32.v nelts < B.length vs);
+       B.upd vs nelts e; vs)
+
+val num_iroots_of: nelts:uint32_t -> Tot uint32_t
+let rec num_iroots_of nelts =
+  admit ()
+  // if nelts = 0ul then 0ul
+  // else 1ul +% num_iroots_of (nelts -% uint32_pow2 (uint32_pow2_floor nelts))
 
 val insert_iroots:
-  nelts:nat{nelts > 0 && nelts < pow2 max_nelts_sz - 1} ->
-  irs:hash_buf{B.length irs = max_nelts_sz} ->
-  nv:elem ->
+  nelts:uint32_t{nelts > 0ul} ->
+  irs:hash_buf ->
+  nv:hash ->
   HST.ST unit
 	 (requires (fun h0 -> B.live h0 irs))
-	 (ensures (fun h0 _ h1 -> modifies (loc_buffer irs) h0 h1))
-	 // TODO: `High.insert_roots` requires values as an argument.
-	 // S.slice (B.as_seq h1 irs) 0 (num_iroots_of_bound max_nelts_sz (insert_nelts nelts)) ==
-	 // High.insert_iroots
-	 //   (S.slice (B.as_seq h0 irs) 0 (num_iroots_of_bound max_nelts_sz nelts)) 
-	 //   (hash_from_elem nv)))
-let rec insert_iroots nirs irs nv =
-  admit ()
+	 (ensures (fun h0 _ h1 -> true))
+#set-options "--z3rlimit 20"
+let rec insert_iroots nelts irs nv =
+  if nelts = 1ul
+  then (assume (B.length irs > 0);
+       hash_from_hashes (B.index irs 0ul) nv (B.index irs 0ul))
+  else if uint32_is_pow2 nelts
+  then B.upd (B.index irs 1ul) 0ul (B.index nv 0ul)
+  else (insert_iroots (nelts -% uint32_pow2 (uint32_pow2_floor nelts))
+  		      (B.sub irs 1ul (num_iroots_of nelts - 1))
+  		      nv;
+       if nelts +% 1ul = uint32_pow2 (uint32_pow2_floor nelts +% 1ul)
+       then hash_from_hashes (B.index irs 0ul) (B.index irs 1ul) 
+       			     (B.index irs 0ul)
+       else ())
 
 val insert: 
-  mt:merkle_tree -> e:elem -> 
+  mt:mtree_ptr -> e:hash -> 
   HST.ST merkle_tree
-	 (requires (fun h0 -> merkle_tree_wf h0 mt /\ ~ (mt_is_full mt)))
-	 (ensures (fun h0 nmt h1 ->
-	   merkle_tree_wf h1 nmt /\
-	   High.insert (merkle_tree_lift h0 mt) e == merkle_tree_lift h1 nmt))
+	 (requires (fun h0 -> true))
+	 (ensures (fun h0 nmt h1 -> true))
 let insert mt e =
   let nnelts = insert_nelts (MT?.nelts mt) in
   let niroots = insert_iroots (MT?.nelts mt) (MT?.iroots mt) e; MT?.iroots mt in
